format-version: 1.2
date: 05:02:2014 02:13
saved-by: danielaraciti
auto-generated-by: OBO-Edit 2.2-rc1
default-namespace: worm_development
ontology: wbls
remark: Version: 1.04
remark: Editors: Wen J. Chen & Daniela Raciti, WormBase, Caltech

[Term]
id: WBls:0000002
name: all stages Ce
def: "All C. elegans development stages, including embryo, larva and adult stage." [wb:wjc]
is_a: WBls:0000075 ! Nematoda Life Stage

[Term]
id: WBls:0000003
name: embryo Ce
def: "The whole period of embryogenesis, from the formation of an egg till its hatch." [wb:wjc]
is_a: WBls:0000002 ! all stages Ce

[Term]
id: WBls:0000004
name: proliferating embryo Ce
def: "0-350min after first cleavage at 20 Centigrade. Proliferate from 1 cell to 560 cells. From start of first cleavage till cleavage is over." [wb:wjc]
is_a: WBls:0000003 ! embryo Ce

[Term]
id: WBls:0000005
name: blastula embryo Ce
def: "0-100min after first cleavage at 20 Centigrade. Proliferate from 1 cell to 28 cells. From first cleavage till the start of gastrulation." [wb:wjc]
is_a: WBls:0000004 ! proliferating embryo Ce

[Term]
id: WBls:0000006
name: 1-cell embryo Ce
def: "Also called zygote. -50min till 0min of first cleavage at 20 Centigrade. Contains 1 cell." [wb:wjc]
is_a: WBls:0000005 ! blastula embryo Ce

[Term]
id: WBls:0000007
name: 2-cell embryo Ce
def: "0-20min after first cleavage at 20 Centigrade.  Contains 2 cells." [wb:wjc]
is_a: WBls:0000005 ! blastula embryo Ce
relationship: preceded_by WBls:0000006 ! 1-cell embryo Ce

[Term]
id: WBls:0000008
name: 4-cell embryo Ce
def: "20-40min after first cleavage at 20 Centigrade.  Contains 4 cells." [wb:wjc]
is_a: WBls:0000005 ! blastula embryo Ce
relationship: preceded_by WBls:0000007 ! 2-cell embryo Ce

[Term]
id: WBls:0000009
name: 28-cell embryo Ce
def: "100-105 min after first cleaveage at 20 Centigrade. Contains 28 cells." [wb:wjc]
is_a: WBls:0000010 ! gastrulating embryo Ce

[Term]
id: WBls:0000010
name: gastrulating embryo Ce
def: "100-290min after first cleavage at 20 Centigrade. Proliferate from 28 cells to 421  cells. Referring to the whole period of gastrulation." [wb:wjc]
is_a: WBls:0000004 ! proliferating embryo Ce
relationship: preceded_by WBls:0000005 ! blastula embryo Ce

[Term]
id: WBls:0000011
name: 51-cell embryo Ce
def: "120-135 min after first cleavage at 20 Centigrade. Contains 51 cells." [wb:wjc]
is_a: WBls:0000010 ! gastrulating embryo Ce
relationship: preceded_by WBls:0000086 ! 44-cell embryo Ce

[Term]
id: WBls:0000012
name: 88-cell embryo Ce
def: "145-150 min after first cleavage at 20 Centigrade. Contains 88 cells." [wb:wjc]
is_a: WBls:0000010 ! gastrulating embryo Ce
relationship: preceded_by WBls:0000088 ! 86-cell embryo Ce

[Term]
id: WBls:0000013
name: enclosing embryo Ce
def: "290-350min after first cleavage at 20 Centigrade. Proliferate from 421 cells to 560 cells. The stage when embryo just finished gastulation and is enclosing." [wb:wjc]
is_a: WBls:0000014 ! late cleavage stage embryo Ce
relationship: preceded_by WBls:0000010 ! gastrulating embryo Ce
relationship: preceded_by WBls:0000014 ! late cleavage stage embryo Ce

[Term]
id: WBls:0000014
name: late cleavage stage embryo Ce
def: "210-350min after first cleavage at 20 Centigrade. Proliferate from 421 cells to 560 cells. The stage before the fast cleavage of cells finishes." [wb:wjc]
is_a: WBls:0000004 ! proliferating embryo Ce
relationship: preceded_by WBls:0000010 ! gastrulating embryo Ce

[Term]
id: WBls:0000015
name: elongating embryo Ce
def: "350-620min after first cleavage at 20 Centigrade. Cell number remains at ~560 cells, with some new cells generated and some cells go through programmed cell death. The stage that embryo starts elongation till elongation is over." [wb:wjc]
is_a: WBls:0000003 ! embryo Ce
relationship: preceded_by WBls:0000004 ! proliferating embryo Ce
relationship: preceded_by WBls:0000010 ! gastrulating embryo Ce

[Term]
id: WBls:0000016
name: bean embryo Ce
def: "350-390min after first cleavage at 20 Centigrade.  Cell number remains at ~560 cells, with some new cells generated and some cells go through programmed cell death. Emrbyo elongation started but have not formed comma shape yet. The shape of embryo looks like a lima bean. A stage right before comma embryo. Also called lima embryo or lima bean stage." [wb:wjc]
is_a: WBls:0000015 ! elongating embryo Ce
relationship: preceded_by WBls:0000013 ! enclosing embryo Ce
relationship: preceded_by WBls:0000014 ! late cleavage stage embryo Ce

[Term]
id: WBls:0000017
name: comma embryo Ce
def: "390-420min after first cleavage at 20 Centigrade. Cell number remains at ~560 cells, with some new cells generated and some cells go through programmed cell death. The shape of embryo looks like a comma. A stage between bean embryo and 1.5-fold embryo." [wb:wjc]
is_a: WBls:0000015 ! elongating embryo Ce
relationship: preceded_by WBls:0000016 ! bean embryo Ce

[Term]
id: WBls:0000018
name: 1.5-fold embryo Ce
def: "420-460min after first cleavage at 20 Centigrade. Cell number remains at ~560 cells, with some new cells generated and some cells go through programmed cell death. The shape of embryo is elongated and fold back 50%. A stage between comma embryo and 2-fold embryo." [wb:wjc]
is_a: WBls:0000015 ! elongating embryo Ce
relationship: preceded_by WBls:0000017 ! comma embryo Ce

[Term]
id: WBls:0000019
name: 2-fold embryo Ce
def: "460-520min after first cleavage at 20 Centigrade. Cell number remains at ~560 cells, with some new cells generated and some cells go through programmed cell death. The shape of embryo is elongated and double fold. A stage between 1.5-fold embryo and 3-fold embryo." [wb:wjc]
is_a: WBls:0000015 ! elongating embryo Ce
relationship: preceded_by WBls:0000018 ! 1.5-fold embryo Ce

[Term]
id: WBls:0000020
name: 3-fold embryo Ce
def: "520-620min after first cleavage at 20 Centigrade. Cell number remains at ~560 cells, with some new cells generated and some cells go through programmed cell death. The shape of embryo is elongated and tripple fold. A stage between 2-fold embryo and fully-elongated embryo. Also called pretzel embryo or pretzel stage." [wb:wjc]
is_a: WBls:0000015 ! elongating embryo Ce
relationship: preceded_by WBls:0000019 ! 2-fold embryo Ce

[Term]
id: WBls:0000021
name: fully-elongated embryo Ce
def: "620-800min(hatch) after first cleavage at 20 Centigrade. Cell number remains at ~560 cells, with some new cells generated and some cells go through programmed cell death. A stage after elongation is over. The last stage of embryogenesis. Also called pre-hatched embryo, late embryo or morphogenetic embryo." [wb:wjc]
is_a: WBls:0000003 ! embryo Ce
relationship: preceded_by WBls:0000015 ! elongating embryo Ce
relationship: preceded_by WBls:0000020 ! 3-fold embryo Ce

[Term]
id: WBls:0000022
name: postembryonic Ce
def: "The stage after hatch till death." [wb:wjc]
is_a: WBls:0000002 ! all stages Ce
relationship: preceded_by WBls:0000003 ! embryo Ce

[Term]
id: WBls:0000023
name: larva Ce
def: "From the time after hatch till becomes adult." [wb:wjc]
is_a: WBls:0000022 ! postembryonic Ce
relationship: preceded_by WBls:0000003 ! embryo Ce

[Term]
id: WBls:0000024
name: L1 larva Ce
def: "The first stage larva. At 25 Centigrade, it ranges 14-25.5 hours after fertilization, 0-11.5 hours after hatch." [wb:wjc]
is_a: WBls:0000023 ! larva Ce
relationship: preceded_by WBls:0000003 ! embryo Ce

[Term]
id: WBls:0000025
name: L1-L2 lethargus Ce
def: "The stage during L1-L2 molt when an animal becomes lethargic, ceases pharyngeal pumping and synthesizes new cuticle under the old." [wb:wjc]
is_a: WBls:0000026 ! L1-L2 molt Ce

[Term]
id: WBls:0000026
name: L1-L2 molt Ce
def: "The stage when an animal shifts from L1 larva to L2 larva. It includes the synthesis of new cuticle, cease of phrayngeal pumping during a lethargus stage, and the shed off of old cuticle." [wb:wjc]
is_a: WBls:0000023 ! larva Ce
relationship: preceded_by WBls:0000024 ! L1 larva Ce

[Term]
id: WBls:0000027
name: L2 larva Ce
def: "The second stage larva. At 25 Centigrade, it ranges 25.5-32.5 hours after fertilization, 11.5-18.5 hours after hatch." [wb:wjc]
is_a: WBls:0000023 ! larva Ce
relationship: preceded_by WBls:0000024 ! L1 larva Ce
relationship: preceded_by WBls:0000026 ! L1-L2 molt Ce

[Term]
id: WBls:0000028
name: L2-L3 lethargus Ce
def: "The stage during L2-L3 molt when an animal becomes lethargic, ceases pharyngeal pumping and synthesizes new cuticle under the old." [wb:wjc]
is_a: WBls:0000029 ! L2-L3 molt Ce

[Term]
id: WBls:0000029
name: L2-L3 molt Ce
def: "The stage when an animal shifts from L2 larva to L3 larva. It includes the synthesis of new cuticle, cease of phrayngeal pumping during a lethargus stage, and the shed off of old cuticle." [wb:wjc]
is_a: WBls:0000023 ! larva Ce
relationship: preceded_by WBls:0000027 ! L2 larva Ce

[Term]
id: WBls:0000030
name: L2d-dauer lethargus Ce
def: "The stage during L2d-dauer molt when an animal becomes lethargic, ceases pharyngeal pumping and synthesizes new cuticle under the old." [wb:wjc]
is_a: WBls:0000031 ! L2d-dauer molt Ce

[Term]
id: WBls:0000031
name: L2d-dauer molt Ce
def: "The stage when an animal shifts from L2d larva to dauer larva. It includes the synthesis of new cuticle, cease of pharyngeal pumping during a lethargus stage, and the shed off of old cuticle." [wb:wjc]
is_a: WBls:0000023 ! larva Ce

[Term]
id: WBls:0000032
name: dauer larva Ce
def: "A third stage larva specialized for dispersal and long term survival." [ISBN:0-87969-433-5]
is_a: WBls:0000023 ! larva Ce
relationship: preceded_by WBls:0000027 ! L2 larva Ce

[Term]
id: WBls:0000033
name: postdauer-L4 lethargus Ce
def: "The stage during postdauer-L4 molt when an animal becomes lethargic, ceases pharyngeal pumping and synthesizes new cuticle under the old." [wb:wjc]
is_a: WBls:0000034 ! postdauer-L4 molt Ce

[Term]
id: WBls:0000034
name: postdauer-L4 molt Ce
def: "The stage when an animal shifts from post dauer stage to L4 larva. It includes the synthesis of new cuticle, cease of phrayngeal pumping during a lethargus stage, and the shed off of old cuticle." [wb:wjc]
is_a: WBls:0000052 ! post dauer stage Ce

[Term]
id: WBls:0000035
name: L3 larva Ce
def: "The third stage larva. At 25 Centigrade, it ranges 32.5-40 hours after fertilization, 18.5-26 hours after hatch." [wb:wjc]
is_a: WBls:0000023 ! larva Ce
relationship: preceded_by WBls:0000027 ! L2 larva Ce
relationship: preceded_by WBls:0000029 ! L2-L3 molt Ce

[Term]
id: WBls:0000036
name: L3-L4 lethargus Ce
def: "The stage during L3-L4 molt when an animal becomes lethargic, ceases pharyngeal pumping and synthesizes new cuticle under the old." [wb:wjc]
is_a: WBls:0000037 ! L3-L4 molt Ce

[Term]
id: WBls:0000037
name: L3-L4 molt Ce
def: "The stage when an animal shifts from L3 larva to L4 larva. It includes the synthesis of new cuticle, cease of phrayngeal pumping during a lethargus stage, and the shed off of old cuticle." [wb:wjc]
is_a: WBls:0000023 ! larva Ce
relationship: preceded_by WBls:0000035 ! L3 larva Ce

[Term]
id: WBls:0000038
name: L4 larva Ce
def: "The fourth stage larva. At 25 Centigrade, it ranges 40-49.5 hours after fertilization, 26-35.5 hours after hatch." [wb:wjc]
is_a: WBls:0000023 ! larva Ce
relationship: preceded_by WBls:0000032 ! dauer larva Ce
relationship: preceded_by WBls:0000035 ! L3 larva Ce
relationship: preceded_by WBls:0000037 ! L3-L4 molt Ce

[Term]
id: WBls:0000039
name: L4-adult lethargus Ce
def: "The stage during L4-adult molt when an animal becomes lethargic, ceases pharyngeal pumping and synthesizes new cuticle under the old." [wb:wjc]
is_a: WBls:0000040 ! L4-adult molt Ce

[Term]
id: WBls:0000040
name: L4-adult molt Ce
def: "The stage when an animal shifts from L4 larva to adult. It includes the synthesis of new cuticle, cease of phrayngeal pumping during a lethargus stage, and the shed off of old cuticle." [wb:wjc]
is_a: WBls:0000023 ! larva Ce
relationship: preceded_by WBls:0000038 ! L4 larva Ce

[Term]
id: WBls:0000041
name: adult Ce
def: "The stage after an animal is fully-developed and reaches maturity." [wb:wjc]
is_a: WBls:0000022 ! postembryonic Ce
relationship: preceded_by WBls:0000023 ! larva Ce
relationship: preceded_by WBls:0000038 ! L4 larva Ce
relationship: preceded_by WBls:0000040 ! L4-adult molt Ce

[Term]
id: WBls:0000042
name: L1-L2 ecdysis Ce
def: "The stage during L1-L2 molt, after the brief lethargus period, when an animal sheds off old cuticle." [wb:wjc]
is_a: WBls:0000026 ! L1-L2 molt Ce
relationship: preceded_by WBls:0000025 ! L1-L2 lethargus Ce

[Term]
id: WBls:0000043
name: L1-L2d molt Ce
def: "The stage when an animal shifts from L1 larva to L2d larva. It includes the synthesis of new cuticle, cease of phrayngeal pumping during a lethargus stage, and the shed off of old cuticle." [wb:wjc]
is_a: WBls:0000023 ! larva Ce

[Term]
id: WBls:0000044
name: L1-L2d lethargus Ce
def: "The stage during L1-L2d molt when an animal becomes lethargic, ceases pharyngeal pumping and synthesizes new cuticle under the old." [wb:wjc]
is_a: WBls:0000043 ! L1-L2d molt Ce

[Term]
id: WBls:0000045
name: L1-L2d ecdysis Ce
def: "The stage during L1-L2d molt, after the brief lethargus period, when an animal sheds off old cuticle." [wb:wjc]
is_a: WBls:0000043 ! L1-L2d molt Ce

[Term]
id: WBls:0000046
name: L2d larva Ce
def: "A special second stage larva with altered physiology and developmental potential that leads to formation of dauer larva. At 25 Centigrade, it ranges 25.5-32.5 hours after fertilization, 11.5-18.5 hours after hatch." [ISBN:0-87969-433-5]
is_a: WBls:0000023 ! larva Ce

[Term]
id: WBls:0000047
name: L2-L3 ecdysis Ce
def: "The stage during L2-L3 molt, after the brief lethargus period, when an animal sheds off old cuticle." [wb:wjc]
is_a: WBls:0000029 ! L2-L3 molt Ce
relationship: preceded_by WBls:0000028 ! L2-L3 lethargus Ce

[Term]
id: WBls:0000048
name: L2d-dauer ecdysis Ce
def: "The stage during L2d-dauer molt, after the brief lethargus period, when an animal sheds off old cuticle." [wb:wjc]
is_a: WBls:0000031 ! L2d-dauer molt Ce

[Term]
id: WBls:0000049
name: L3-L4 ecdysis Ce
def: "The stage during L3-L4 molt, after the brief lethargus period, when an animal sheds off old cuticle." [wb:wjc]
is_a: WBls:0000037 ! L3-L4 molt Ce
relationship: preceded_by WBls:0000036 ! L3-L4 lethargus Ce

[Term]
id: WBls:0000050
name: L4-adult ecdysis
def: "The stage during L4-adult molt, after the brief lethargus period, when an animal shed off old cuticle." [wb:wjc]
is_a: WBls:0000040 ! L4-adult molt Ce
relationship: preceded_by WBls:0000039 ! L4-adult lethargus Ce

[Term]
id: WBls:0000051
name: postdauer-L4 ecdysis Ce
def: "The stage during postdauer-L4 molt, after the brief lethargus period, when an animal sheds off old cuticle." [wb:wjc]
is_a: WBls:0000034 ! postdauer-L4 molt Ce

[Term]
id: WBls:0000052
name: post dauer stage Ce
def: "The stage right after an animal recovered from dauer but has not started transformation to L4 larva yet." [wb:wjc]
is_a: WBls:0000023 ! larva Ce

[Term]
id: WBls:0000053
name: L2d-L3 molt Ce
def: "The stage when an animal shifts from L2d larva to L3 larva. It includes the synthesis of new cuticle, cease of phrayngeal pumping during a lethargus stage, and the shed off of old cuticle." [wb:wjc]
is_a: WBls:0000046 ! L2d larva Ce

[Term]
id: WBls:0000054
name: L2d-L3 lethargus Ce
def: "The stage during L2d-L3 molt when an animal becomes lethargic, ceases pharyngeal pumping and synthesizes new cuticle under the old." [wb:wjc]
is_a: WBls:0000053 ! L2d-L3 molt Ce

[Term]
id: WBls:0000055
name: L2d-L3 ecdysis Ce
def: "The stage during L2d-L3 molt, after the brief lethargus period, when an animal sheds off old cuticle." [wb:wjc]
is_a: WBls:0000053 ! L2d-L3 molt Ce

[Term]
id: WBls:0000056
name: adult male Ce
def: "The stage after an male animal is fully-developed and reaches maturity." [wb:wjc]
is_a: WBls:0000041 ! adult Ce

[Term]
id: WBls:0000057
name: adult hermaphrodite Ce
def: "The stage after an hermaphrodite animal is fully-developed and reaches maturity." [wb:wjc]
is_a: WBls:0000041 ! adult Ce

[Term]
id: WBls:0000058
name: pre-reproductive stage adult hermaphrodite Ce
def: "Very young adult hermaphrodites that do not have eggs in the uterus yet. At 20 Centigrade: 0 - 13 hours after L4-adult molt. 3 days after first cleaveage." [wb:wjc]
is_a: WBls:0000057 ! adult hermaphrodite Ce

[Term]
id: WBls:0000060
name: reproductive stage adult hermaphrodite Ce
def: "Adult hermaphrodites continuously laying fertilized eggs. Hermaphrodite in egg laying stages--usually up to 4/5 days after L4-adult molt at Centigrade. From the first fertilized egg is laid, till all sperms are used. At 20 Centigrade: 13 hours after L4-adult molt until about 5.4 days after the L4-adult molt. 3-8.4 days after first cleavage." [wb:wjc]
is_a: WBls:0000057 ! adult hermaphrodite Ce

[Term]
id: WBls:0000061
name: oocyte-laying stage adult hermaphrodite Ce
def: "When egg-laying is still going on but intermittent and during which a significant number of oocytes are laid. Included in reproductive stage adult hermaphrodite." [wb:wjc]
is_a: WBls:0000057 ! adult hermaphrodite Ce

[Term]
id: WBls:0000062
name: post-reproductive stage adult hermaphrodite Ce
def: "Adult hermaphrodites that contain no more sperm, thus stop egg-laying, but still alive. At 20 Centigrade: 5.4 days after L4-adult molt until the death. 8.4 - 13.2 (average wild type life span) days after first cleavage." [wb:wjc]
is_a: WBls:0000057 ! adult hermaphrodite Ce

[Term]
id: WBls:0000063
name: newly molted young adult hermaphrodite Ce
def: "At 20 Centigrade: 0-24 hours after L4-adult molt." [wb:wjc]
is_a: WBls:0000057 ! adult hermaphrodite Ce

[Term]
id: WBls:0000064
name: 1-day post-L4 adult hermaphrodite Ce
def: "At 20 Centigrade: 24-48 hours after L4-adult molt. 4-5 days after first cleavage." [wb:wjc]
is_a: WBls:0000057 ! adult hermaphrodite Ce

[Term]
id: WBls:0000065
name: 2-days post-L4 adult hermaphrodite Ce
def: "At 20 Centigrade: 48-72 hours after L4-adult molt. 5-6 days after first cleavage." [wb:wjc]
is_a: WBls:0000057 ! adult hermaphrodite Ce
relationship: preceded_by WBls:0000064 ! 1-day post-L4 adult hermaphrodite Ce

[Term]
id: WBls:0000066
name: 3-days post-L4 adult hermaphrodite Ce
def: "At 20 Centigrade: 72-96 hours after L4-adult molt. 6-7 days after first cleavage." [wb:wjc]
is_a: WBls:0000057 ! adult hermaphrodite Ce
relationship: preceded_by WBls:0000065 ! 2-days post-L4 adult hermaphrodite Ce

[Term]
id: WBls:0000067
name: 4-days post-L4 adult hermaphrodite Ce
def: "At 20 Centigrade: 96-120 hours after L4-adult molt. 7-8 days after first cleavage." [wb:wjc]
is_a: WBls:0000057 ! adult hermaphrodite Ce
relationship: preceded_by WBls:0000066 ! 3-days post-L4 adult hermaphrodite Ce

[Term]
id: WBls:0000068
name: 5-days post-L4 adult hermaphrodite Ce
def: "At 20 Centigrade: 5-6 days after L4-adult molt. 8-9 days after first cleavage." [wb:wjc]
is_a: WBls:0000057 ! adult hermaphrodite Ce
relationship: preceded_by WBls:0000067 ! 4-days post-L4 adult hermaphrodite Ce

[Term]
id: WBls:0000069
name: 4-7 days post-L4 adult hermaphrodite Ce
def: "At 20 Centigrade: 4-7 days after L4-adult molt. 7-10 days after first cleavage." [wb:wjc]
is_a: WBls:0000057 ! adult hermaphrodite Ce
relationship: preceded_by WBls:0000068 ! 5-days post-L4 adult hermaphrodite Ce

[Term]
id: WBls:0000070
name: 7-10 days post-L4 adult hermaphrodite Ce
def: "At 20 Centigrade: 7-10 days after L4-adult molt. 10-13 days after first cleavage." [wb:wjc]
is_a: WBls:0000057 ! adult hermaphrodite Ce
relationship: preceded_by WBls:0000069 ! 4-7 days post-L4 adult hermaphrodite Ce

[Term]
id: WBls:0000071
name: 8-cell embryo Ce
def: "~50 min after first cleavage at 20 Centigrade.  Contains 8 cells." [wb:wjc]
is_a: WBls:0000005 ! blastula embryo Ce
relationship: preceded_by WBls:0000008 ! 4-cell embryo Ce

[Term]
id: WBls:0000072
name: 12-cell embryo Ce
def: "~55 min after first cleavage at 20 Centigrade.  Contains 12 cells." [wb:wjc]
is_a: WBls:0000005 ! blastula embryo Ce
relationship: preceded_by WBls:0000071 ! 8-cell embryo Ce

[Term]
id: WBls:0000073
name: L4 larva male Ce
def: "The fourth stage larva male. At 25 Centigrade, it ranges 40-49.5 hours after fertilization, 26-35.5 hours after hatch." [wb:wjc]
is_a: WBls:0000038 ! L4 larva Ce

[Term]
id: WBls:0000074
name: 11-15 days post-L4 adult hermaphrodite Ce
def: "At 20 Centigrade: 11-15 days after L4-adult molt. 14-18 days after first cleavage." [wb:dr]
is_a: WBls:0000057 ! adult hermaphrodite Ce
relationship: preceded_by WBls:0000070 ! 7-10 days post-L4 adult hermaphrodite Ce
created_by: danielaraciti
creation_date: 2012-05-22T14:35:04Z

[Term]
id: WBls:0000075
name: Nematoda Life Stage
created_by: danielaraciti
creation_date: 2012-05-30T09:04:28Z

[Term]
id: WBls:0000077
name: sheathed microfilaria Bma
def: "Microfilaria is the stage which develops from the egg and precedes the L1 stage. The larvae are surrounded by a membrane thought to be derived from the vitelline membrane." [wb:dr&mb]
synonym: "microfilaria" EXACT []
is_a: WBls:0000097 ! larva Bma
created_by: danielaraciti
creation_date: 2012-05-30T09:23:44Z

[Term]
id: WBls:0000079
name: L1 larva Bma
alt_id: WBls:0000078
def: "The first stage larva. Also known as vector-derived microfilaria. The microfilaria sheds the sheath and matures to a 'proper L1' in the bloodmeal in the vector gut, and then migrates to the muscles." [WB:dr&mb]
synonym: "unsheathed microfilaria Bma" EXACT []
is_a: WBls:0000097 ! larva Bma
relationship: preceded_by WBls:0000077 ! sheathed microfilaria Bma
created_by: danielaraciti
creation_date: 2012-05-30T09:29:36Z

[Term]
id: WBls:0000080
name: L2 larva Bma
def: "The second stage larva. Derived from flight muscles of vector host; some development in vitro, with L1 to L2 moulting, has been demonstrated but rarely; these are often staged by hours or days post blood meal." [wb:dr&mb]
is_a: WBls:0000097 ! larva Bma
relationship: preceded_by WBls:0000079 ! L1 larva Bma
created_by: danielaraciti
creation_date: 2012-05-30T09:30:40Z

[Term]
id: WBls:0000081
name: L3 larva Bma
def: "The third stage larva." [wb:dr&mb]
is_a: WBls:0000097 ! larva Bma
relationship: preceded_by WBls:0000080 ! L2 larva Bma
created_by: danielaraciti
creation_date: 2012-05-30T09:31:06Z

[Term]
id: WBls:0000082
name: L4 larva Bma
def: "The fourth stage larva. Should be conditioned by days post infection; as moulting is not synchronous, some samples are defined as L3/L4, indicating a mix of individuals as late L3, moulting, and early L4." [wb:dr&mb]
is_a: WBls:0000097 ! larva Bma
relationship: preceded_by WBls:0000081 ! L3 larva Bma
created_by: danielaraciti
creation_date: 2012-05-30T09:31:38Z

[Term]
id: WBls:0000083
name: adult Bma
def: "Adults (or at least adult females) can live for 10 years in a human host, and can outlive their rodent laboratory hosts; it is usual to state the chronological age of the nematodes in days or months post-infection, and occasionally post-patency (the production of first microfilariae)." [WB:dr&mb]
is_a: WBls:0000093 ! postembryonic Bma
relationship: preceded_by WBls:0000100 ! young adult Bma
created_by: danielaraciti
creation_date: 2012-05-30T09:32:18Z

[Term]
id: WBls:0000084
name: 14-cell embryo Ce
def: "E-cell has divided into Ea and Ep. Contains 14 cells." [wb:dr]
comment: Levin M, Hashimshony T, Wagner F, Yanai I. Developmental milestones punctuate gene expression in the Caenorhabditis embryo. Dev Cell. 2012 May 15;22(5):1101-8. Epub 2012 May 3. PubMed PMID: 22560298. Supplementary table 1.
is_a: WBls:0000005 ! blastula embryo Ce
relationship: preceded_by WBls:0000072 ! 12-cell embryo Ce
created_by: danielaraciti
creation_date: 2012-10-02T17:15:41Z

[Term]
id: WBls:0000085
name: 24-cell embryo Ce
def: "Fourth cleavage of the AB lineage. Contains 24 cells." [wb:dr]
comment: Levin M, Hashimshony T, Wagner F, Yanai I. Developmental milestones punctuate gene expression in the Caenorhabditis embryo. Dev Cell. 2012 May 15;22(5):1101-8. Epub 2012 May 3. PubMed PMID: 22560298. Supplementary table 1.
is_a: WBls:0000005 ! blastula embryo Ce
relationship: preceded_by WBls:0000084 ! 14-cell embryo Ce
created_by: danielaraciti
creation_date: 2012-10-02T17:23:32Z

[Term]
id: WBls:0000086
name: 44-cell embryo Ce
def: "Fifth cleavage of the AB lineage. Contains 44 cells." [wb:dr]
comment: Levin M, Hashimshony T, Wagner F, Yanai I. Developmental milestones punctuate gene expression in the Caenorhabditis embryo. Dev Cell. 2012 May 15;22(5):1101-8. Epub 2012 May 3. PubMed PMID: 22560298. Supplementary table 1.
is_a: WBls:0000010 ! gastrulating embryo Ce
relationship: preceded_by WBls:0000009 ! 28-cell embryo Ce
created_by: danielaraciti
creation_date: 2012-10-02T17:25:18Z

[Term]
id: WBls:0000087
name: 68-cell embryo Ce
def: "Sixth cleavage of the AB lineage. Contains 68 cells." [wb:dr]
comment: Levin M, Hashimshony T, Wagner F, Yanai I. Developmental milestones punctuate gene expression in the Caenorhabditis embryo. Dev Cell. 2012 May 15;22(5):1101-8. Epub 2012 May 3. PubMed PMID: 22560298. Supplementary table 1.
is_a: WBls:0000010 ! gastrulating embryo Ce
relationship: preceded_by WBls:0000011 ! 51-cell embryo Ce
created_by: danielaraciti
creation_date: 2012-10-02T17:26:52Z

[Term]
id: WBls:0000088
name: 86-cell embryo Ce
def: "Seventh cleavage of the AB lineage. Contains 86 cells." [wb:dr]
comment: Levin M, Hashimshony T, Wagner F, Yanai I. Developmental milestones punctuate gene expression in the Caenorhabditis embryo. Dev Cell. 2012 May 15;22(5):1101-8. Epub 2012 May 3. PubMed PMID: 22560298. Supplementary table 1.
is_a: WBls:0000010 ! gastrulating embryo Ce
relationship: preceded_by WBls:0000087 ! 68-cell embryo Ce
created_by: danielaraciti
creation_date: 2012-10-02T17:27:50Z

[Term]
id: WBls:0000089
name: 190-cells embryo Ce
def: "P4 and M cells have finished migrating. Contains 190 cells." [wb:dr]
is_a: WBls:0000010 ! gastrulating embryo Ce
relationship: preceded_by WBls:0000090 ! 96-cell embryo Ce
created_by: danielaraciti
creation_date: 2012-10-15T13:19:10Z

[Term]
id: WBls:0000090
name: 96-cell embryo Ce
def: "155-165 min after first cleavage at 20 Centigrade. Contains 96 cells." [wb:dr]
is_a: WBls:0000010 ! gastrulating embryo Ce
relationship: preceded_by WBls:0000012 ! 88-cell embryo Ce
created_by: danielaraciti
creation_date: 2012-10-16T15:37:30Z

[Term]
id: WBls:0000091
name: all stages Bma
def: "All B. malayi developmental stages, including embryo, larva and adult stage." [wb:dr&mb]
is_a: WBls:0000075 ! Nematoda Life Stage
created_by: danielaraciti
creation_date: 2013-11-12T03:18:57Z

[Term]
id: WBls:0000092
name: embryo Bma
def: "The whole period of embryogenesis, from the formation of an egg till its hatch." [WB:dr]
is_a: WBls:0000091 ! all stages Bma
created_by: danielaraciti
creation_date: 2013-11-12T04:48:28Z

[Term]
id: WBls:0000093
name: postembryonic Bma
def: "The stage after hatch till death." [WB:dr]
is_a: WBls:0000091 ! all stages Bma
relationship: preceded_by WBls:0000092 ! embryo Bma
created_by: danielaraciti
creation_date: 2013-11-12T04:50:29Z

[Term]
id: WBls:0000094
name: early embryo Bma
def: "Proliferates from 1 to 100 cells. As the Brugia female reproductive tract is long (>10 cm), it is possible to dissect it and select early embryos just by isolating early parts of the post-spermatheca uterus." [WB:dr&mb]
is_a: WBls:0000092 ! embryo Bma
created_by: danielaraciti
creation_date: 2013-11-12T04:55:53Z

[Term]
id: WBls:0000095
name: middle embryo Bma
def: "Proliferates from 100 cells to Lima bean stage." [WB:dr&mb]
is_a: WBls:0000092 ! embryo Bma
relationship: preceded_by WBls:0000094 ! early embryo Bma
created_by: danielaraciti
creation_date: 2013-11-12T04:59:19Z

[Term]
id: WBls:0000096
name: late embryo Bma
def: "From Lima bean to hatching." [WB:dr&mb]
is_a: WBls:0000092 ! embryo Bma
relationship: preceded_by WBls:0000095 ! middle embryo Bma
created_by: danielaraciti
creation_date: 2013-11-12T05:00:28Z

[Term]
id: WBls:0000097
name: larva Bma
def: "From the time after hatch till becomes adult." [WB:dr]
is_a: WBls:0000093 ! postembryonic Bma
relationship: preceded_by WBls:0000092 ! embryo Bma
created_by: danielaraciti
creation_date: 2013-11-12T05:12:19Z

[Term]
id: WBls:0000098
name: vector-derived L3 Bma
def: "Also known as infective L3, or iL3; i.e. isolated from the vector salivary glands; these samples may-should be conditioned by age, which is usually counted in days from the blood meal." [wb:dr&mb]
synonym: "iL3" RELATED []
synonym: "infective L3" RELATED []
is_a: WBls:0000081 ! L3 larva Bma
created_by: danielaraciti
creation_date: 2013-11-12T05:23:54Z

[Term]
id: WBls:0000099
name: post-infection L3 Bma
def: "Derived from the host after reintroduction by vector feeding or manual inoculation; these piL3 samples are often-should be conditioned by age (hours or days post-infection)." [wb:dr&mb]
synonym: "piL3" RELATED []
is_a: WBls:0000081 ! L3 larva Bma
created_by: danielaraciti
creation_date: 2013-11-12T05:24:59Z

[Term]
id: WBls:0000100
name: young adult Bma
def: "The animals have a significant \"prepatent\" period in the host, where they have moulted to adults but not yet started producing eggs or sperm; this stage is usually-should be conditioned by days post infection, with day 26 to approximately day 60 being the \"young adult\" in most systems - but note that the speed of development is different in different host genotypes." [wb:dr&mb]
is_a: WBls:0000093 ! postembryonic Bma
relationship: preceded_by WBls:0000082 ! L4 larva Bma
created_by: danielaraciti
creation_date: 2013-11-12T05:37:52Z

[Term]
id: WBls:0000101
name: all stages nematode
def: "All developmental stages, including embryo, larva and adult stage." [wb:dr]
is_a: WBls:0000075 ! Nematoda Life Stage
created_by: danielaraciti
creation_date: 2013-11-25T06:13:37Z

[Term]
id: WBls:0000102
name: embryo nematode
def: "The whole period of embryogenesis, from the formation of an egg till its hatch." [wb:dr]
is_a: WBls:0000101 ! all stages nematode
created_by: danielaraciti
creation_date: 2013-11-25T06:14:14Z

[Term]
id: WBls:0000103
name: postembryonic nematode
def: "The stage after hatch till death." [wb:dr]
is_a: WBls:0000101 ! all stages nematode
relationship: preceded_by WBls:0000102 ! embryo nematode
created_by: danielaraciti
creation_date: 2013-11-25T06:14:39Z

[Term]
id: WBls:0000104
name: adult nematode
def: "The stage after an animal is fully-developed and reaches maturity." [wb:dr]
is_a: WBls:0000103 ! postembryonic nematode
relationship: preceded_by WBls:0000105 ! larva nematode
created_by: danielaraciti
creation_date: 2013-11-25T06:18:53Z

[Term]
id: WBls:0000105
name: larva nematode
def: "From the time after hatch till becomes adult." [wb:dr]
is_a: WBls:0000103 ! postembryonic nematode
created_by: danielaraciti
creation_date: 2013-11-25T06:19:27Z

[Term]
id: WBls:0000106
name: L1 larva nematode
def: "The first stage larva." [wb:dr]
is_a: WBls:0000105 ! larva nematode
relationship: preceded_by WBls:0000110 ! sheathed microfilaria nematode
created_by: danielaraciti
creation_date: 2013-11-25T06:20:28Z

[Term]
id: WBls:0000107
name: L2 larva nematode
def: "The second stage larva." [wb:dr]
is_a: WBls:0000105 ! larva nematode
relationship: preceded_by WBls:0000106 ! L1 larva nematode
created_by: danielaraciti
creation_date: 2013-11-25T06:20:54Z

[Term]
id: WBls:0000108
name: L3 larva nematode
def: "The third stage larva." [wb:dr]
is_a: WBls:0000105 ! larva nematode
relationship: preceded_by WBls:0000107 ! L2 larva nematode
created_by: danielaraciti
creation_date: 2013-11-25T06:21:33Z

[Term]
id: WBls:0000109
name: L4 larva nematode
def: "The fourth stage larva." [wb:dr]
is_a: WBls:0000105 ! larva nematode
relationship: preceded_by WBls:0000108 ! L3 larva nematode
created_by: danielaraciti
creation_date: 2013-11-25T06:22:48Z

[Term]
id: WBls:0000110
name: sheathed microfilaria nematode
def: "Microfilaria is the stage which develops from the egg and precedes the L1 stage. The larvae are surrounded by a membrane thought to be derived from the vitelline membrane." [wb:dr]
is_a: WBls:0000105 ! larva nematode
created_by: danielaraciti
creation_date: 2013-11-25T06:23:23Z

[Term]
id: WBls:0000111
name: 16-18 days post-L4 adult hermaphrodite Ce
def: "At 20 Centigrade: 16-18 days after L4-adult molt. 18-21 days after first cleavage." [wb:dr]
is_a: WBls:0000057 ! adult hermaphrodite Ce
relationship: preceded_by WBls:0000074 ! 11-15 days post-L4 adult hermaphrodite Ce
created_by: danielaraciti

[Typedef]
id: part_of
name: part of
xref: BFO:0000050
is_transitive: true

[Typedef]
id: preceded_by
name: preceded_by
xref: BFO:0000062
is_transitive: true

